getval tests

src/Compiler/Compiler.v
@@ -81,20 +81,93 @@ Definition alist_sub (m1 m2 : alist string unit) : alist string unit :=
 fold_alist sub m1 m2.
  *)
 
-Fixpoint gen_body_code (p : AST.stmt) : code dtyp :=
+Definition gen_body_code (p : AST.stmt) : code dtyp :=
   match p with
   | Skip => nil
   | Assign x v => match v with 
-                  | Lit n => [(IVoid 0%Z, (INSTR_Store false ((DTYPE_I 32%N), (EXP_Integer (Int32.unsigned n))) (DTYPE_Pointer, (EXP_Ident (ID_Local (Name x)))) None))]
-                  end
+                  | Lit n => [(IId (Anon 0%Z), (INSTR_Op (EXP_Integer (Int32.unsigned n))))]
+                  | Var x => [(IId (Anon 0%Z), (INSTR_Load false (DTYPE_I 32%N) (DTYPE_Pointer, (EXP_Ident (ID_Local (Name x)))) None))]
+  end ++ [(IVoid 0%Z, (INSTR_Store false ((DTYPE_I 32%N), (EXP_Ident (ID_Local (Anon 0%Z)))) (DTYPE_Pointer, (EXP_Ident (ID_Local (Name x)))) None))]
   end.
 
 
-Fixpoint compile (p : AST.prog) : code dtyp :=
+Fixpoint compile_aux (p : AST.prog) : code dtyp :=
   match p with
   | nil => nil
-  | x :: t => (gen_body_code x) ++ (compile t)
+  | x :: t => (gen_body_code x) ++ (compile_aux t)
   end.
+
+Definition compile (p : AST.prog) : code dtyp :=
+  compile_aux p.
+
+
+Definition extract_z_instr_id (ins:instr_id) : Z :=
+  match ins with
+  | IId r => match r with
+             | Anon z => z
+             | _ => -1%Z
+             end
+  | _ => -1%Z
+  end.
+
+Definition extract_z_ident (id:ident) : Z :=
+  match id with
+  | ID_Local r => match r with
+                  | Anon z => z
+                  | _ => -1%Z
+                  end
+  | _ => -1%Z
+  end.
+
+
+Fixpoint replace_exp (e : exp dtyp) (map : FMapAList.alist Z Z) :=
+  match e with
+  | EXP_Ident id => match FMapAList.alist_find (extract_z_ident id) map with
+                    | Some v => EXP_Ident (ID_Local (Anon v))
+                    | None => e
+                    end
+  | OP_IBinop v1 v2 e1 e2 => OP_IBinop v1 v2 (replace_exp e1 map) (replace_exp e2 map)
+  | _ => e
+  end.
+
+
+
+Definition replace_inst (ib : instr dtyp) (map : FMapAList.alist Z Z) : instr dtyp :=
+  match ib with
+  | INSTR_Op e => INSTR_Op (replace_exp e map)
+  | INSTR_Store v (t, e1) (t2, e2) a => INSTR_Store v (t, (replace_exp e1 map)) (t2, e2) a
+  | _ => ib
+  end.
+
+
+Definition replace_id (id: instr_id) (map : FMapAList.alist Z Z) : instr_id :=
+  match id with
+  | IId r => match r with
+             | Anon z => match FMapAList.alist_find (extract_z_instr_id id) map with
+                         | Some v => IId (Anon v)
+                         | None => id
+                         end
+             | _ => id
+             end
+  | _ => id
+  end.
+
+
+Fixpoint ssa (input : code dtyp) (map : FMapAList.alist Z Z) (c : Z): code dtyp :=
+  match input with
+  | nil => nil
+  | h :: t => let '(id, ib) := h in
+              let zid := extract_z_instr_id id in
+              let ib' := replace_inst ib map in
+              let map' := if (zid =? (-1%Z))%Z then map else (match FMapAList.alist_find zid map with | Some v => FMapAList.alist_add zid c map | None => FMapAList.alist_add zid zid map end) in
+              let c'   := if (zid =? (-1%Z))%Z then c else (match FMapAList.alist_find zid map with | Some v => (c + 1)%Z | None => c end) in
+              let id'  := replace_id id map' in
+                (id', ib') :: (ssa t map' c')
+  end.
+
+
+
+Compute ssa (compile ([Assign "x" (Lit (Int32.repr 5%Z));Assign "y" (Lit (Int32.repr 3%Z));Assign "x" (Var "x")])) ([]) (1%Z).
 
 
 
